Update Float->SymFloat translation properites, proofs

coq/FSigmaHCOL/FHCOLtoLFHCOL.v
@@ -22,12 +22,14 @@ Module Export FHCOLtoLFHCOL := MDHCOLTypeTranslator
                                  (FHCOLEval)
                                  (LFHCOLEval).
 
-Inductive heq_Float_SymFloat : MFloat64asCT.t -> MLazyFloat64asCT.t -> Prop :=
-| heq_FSF_Some : forall f sf,
-    evalSymFloat sf ≡ Some f -> heq_Float_SymFloat f sf
-| heq_FSF_None : forall f, heq_Float_SymFloat f None.
+Definition heq_Float_SymFloat
+  (env : FloatEnv)
+  (f : MFloat64asCT.t)
+  (sf : MLazyFloat64asCT.t)
+  : Prop :=
+  evalFloatExpr env sf ≡ Some f.
 
-Global Instance FLF_CHE : FHCOLtoLFHCOL.CTranslation_heq.
+Global Instance FLF_CHE : FHCOLtoLFHCOL.CTranslation_heq FloatEnv.
 Proof.
   econstructor.
   -
@@ -36,134 +38,19 @@ Proof.
     invc F; invc LF.
     easy.
   -
-    intros * T.
+    intros * T *.
     unfold translateCTypeConst in *.
     repeat break_if; invc T.
-    all: rewrite e.
-    all: constructor.
-    all: now rewrite <-H1.
+    all: now rewrite e, <-H1.
 Defined.
 
-Global Instance FLF_COP : @FHCOLtoLFHCOL.COpTranslationProps FLF_CHE.
+Global Instance FLF_COP : @FHCOLtoLFHCOL.COpTranslationProps FloatEnv FLF_CHE.
 Proof.
   do 2 constructor.
   all: intros * XE; try intro YE.
-  -
-    inversion XE as [t1 t2 EX t3 t4| t1 t2 EX]; clear XE; subst;
-      inversion YE as [t1 t2 EY t3 t4| t1 t2 EY]; clear YE; subst.
-    2-4: cbn; repeat break_match; constructor 2.
-    destruct x' as [[xe xf] |],
-             y' as [[ye yf] |]; try some_none.
-    all: cbn in *.
-    2-4: constructor 2.
-    all: destruct (List.list_eq_dec MFloat64asCT.CTypeEquivDec xe ye)
-      as [EEQ | ENEQ].
-    all: repeat break_match; subst.
-    6: constructor 2.
-    all: constructor; cbn.
-    all: rewrite ?EX, ?EY.
-    all: try erewrite evalFloatExpr_env_indep by eassumption.
-    all: try reflexivity.
-    now rewrite EEQ, EY.
-  -
-    inversion XE as [t1 t2 EX t3 t4| t1 t2 EX]; clear XE; subst;
-      inversion YE as [t1 t2 EY t3 t4| t1 t2 EY]; clear YE; subst.
-    2-4: cbn; repeat break_match; constructor 2.
-    destruct x' as [[xe xf] |],
-             y' as [[ye yf] |]; try some_none.
-    all: cbn in *.
-    2-4: constructor 2.
-    all: destruct (List.list_eq_dec MFloat64asCT.CTypeEquivDec xe ye)
-      as [EEQ | ENEQ].
-    all: repeat break_match; subst.
-    6: constructor 2.
-    all: constructor; cbn.
-    all: rewrite ?EX, ?EY.
-    all: try erewrite evalFloatExpr_env_indep by eassumption.
-    all: try reflexivity.
-    now rewrite EEQ, EY.
-  -
-    inversion XE as [t1 t2 EX t3 t4| t1 t2 EX]; clear XE; subst;
-      inversion YE as [t1 t2 EY t3 t4| t1 t2 EY]; clear YE; subst.
-    2-4: cbn; repeat break_match; constructor 2.
-    destruct x' as [[xe xf] |],
-             y' as [[ye yf] |]; try some_none.
-    all: cbn in *.
-    2-4: constructor 2.
-    all: destruct (List.list_eq_dec MFloat64asCT.CTypeEquivDec xe ye)
-      as [EEQ | ENEQ].
-    all: repeat break_match; subst.
-    6: constructor 2.
-    all: constructor; cbn.
-    all: rewrite ?EX, ?EY.
-    all: try erewrite evalFloatExpr_env_indep by eassumption.
-    all: try reflexivity.
-    now rewrite EEQ, EY.
-  -
-    inversion XE as [t1 t2 EX t3 t4| t1 t2 EX]; clear XE; subst;
-      inversion YE as [t1 t2 EY t3 t4| t1 t2 EY]; clear YE; subst.
-    2-4: cbn; repeat break_match; constructor 2.
-    destruct x' as [[xe xf] |],
-             y' as [[ye yf] |]; try some_none.
-    all: cbn in *.
-    2-4: constructor 2.
-    all: destruct (List.list_eq_dec MFloat64asCT.CTypeEquivDec xe ye)
-      as [EEQ | ENEQ].
-    all: repeat break_match; subst.
-    6: constructor 2.
-    all: constructor; cbn.
-    all: rewrite ?EX, ?EY.
-    all: try erewrite evalFloatExpr_env_indep by eassumption.
-    all: try reflexivity.
-    now rewrite EEQ, EY.
-  -
-    inversion XE as [t1 t2 EX t3 t4| t1 t2 EX]; clear XE; subst;
-      inversion YE as [t1 t2 EY t3 t4| t1 t2 EY]; clear YE; subst.
-    2-4: cbn; repeat break_match; constructor 2.
-    destruct x' as [[xe xf] |],
-             y' as [[ye yf] |]; try some_none.
-    all: cbn in *.
-    2-4: constructor 2.
-    all: destruct (List.list_eq_dec MFloat64asCT.CTypeEquivDec xe ye)
-      as [EEQ | ENEQ].
-    all: repeat break_match; subst.
-    6: constructor 2.
-    all: constructor; cbn.
-    all: rewrite ?EX, ?EY.
-    all: try erewrite evalFloatExpr_env_indep by eassumption.
-    all: try reflexivity.
-    now rewrite EEQ, EY.
-  -
-    inversion XE as [t1 t2 EX t3 t4| t1 t2 EX]; clear XE; subst;
-      inversion YE as [t1 t2 EY t3 t4| t1 t2 EY]; clear YE; subst.
-    2-4: cbn; repeat break_match; constructor 2.
-    destruct x' as [[xe xf] |],
-             y' as [[ye yf] |]; try some_none.
-    all: cbn in *.
-    2-4: constructor 2.
-    all: destruct (List.list_eq_dec MFloat64asCT.CTypeEquivDec xe ye)
-      as [EEQ | ENEQ].
-    all: repeat break_match; subst.
-    6: constructor 2.
-    all: constructor; cbn.
-    all: rewrite ?EX, ?EY.
-    all: try erewrite evalFloatExpr_env_indep by eassumption.
-    all: try reflexivity.
-    now rewrite EEQ, EY.
-  -
-    inversion XE as [t1 t2 EX t3 t4| t1 t2 EX]; clear XE; subst.
-    2: constructor 2.
-    destruct x' as [[xe xf] |]; try some_none.
-    2: constructor 2.
-    constructor; cbn in *.
-    now rewrite EX.
-  -
-    inversion XE as [t1 t2 EX t3 t4| t1 t2 EX]; clear XE; subst.
-    2: constructor 2.
-    destruct x' as [[xe xf] |]; try some_none.
-    2: constructor 2.
-    constructor; cbn in *.
-    now rewrite EX.
+  all: unfold heq_CType', FLF_CHE, heq_Float_SymFloat in *.
+  all: cbn.
+  all: now rewrite ?XE, ?YE.
 Qed.
 
 (* Trivial instances for "translating" Int64 -> Int64 *)
